Flows/Herbrand.lean
@@ -1,0 +1,551 @@
+/-
+Copyright (c) 2021-2022 Julien Marquet. All rights reserved.
+Released under Apache 2.0 license as described in the file LICENSE.
+Authors: Julien Marquet
+-/
+
+import Lean
+
+import Flows.Groundwork
+import Flows.SolveSets
+import Flows.Term
+import Flows.Subst
+import Flows.Vehicle
+import Flows.Vanishing
+import Flows.Unifier
+
+open Classical
+
+set_option codegen false
+
+universe u
+
+section
+
+theorem cons_carrier_in {θ φ : Subst α β} {l₁ r₁ l₂ r₂ : Term α β}
+  (h₁ : (𝒱 θ : Fintype β) ⊆ 𝒱 l₁ ∪ 𝒱 l₂)
+  (h₂ : (𝒱 φ : Fintype β) ⊆ 𝒱 (r₁ • θ) ∪ 𝒱 (r₂ • θ))
+  (h₃ : vanishing θ) (h₄ : vanishing φ)
+  (h₅ : carrier θ ⊆ 𝒱 l₁ ∪ 𝒱 l₂) (h₆ : carrier φ ⊆ 𝒱 (r₁ • θ) ∪ 𝒱 (r₂ • θ)) :
+  carrier (θ * φ) ⊆ 𝒱 (Term.Cons l₁ r₁) ∪ 𝒱 (Term.Cons l₂ r₂) := by
+  apply Fintype.included_trans (carrier_cons _ _)
+  simp only [vehicle_cons]
+  rw [Fintype.union_assoc]
+  apply Fintype.union_included_iff.2 (And.intro _ _)
+  focus
+    apply Fintype.included_trans h₅
+    solve_sets
+  focus
+    apply Fintype.included_trans h₆
+    apply Fintype.union_included_iff.2 ⟨ _, _ ⟩
+      <;> apply Fintype.included_trans (vehicle_on_image h₁ _)
+      <;> solve_sets
+
+end
+
+section
+
+theorem lex_of_le_and_lt {α β : Type u}
+  {ha : WellFoundedRelation α} {hb : WellFoundedRelation β}
+  {a₁ a₂ : α} {b₁ b₂ : β} (h₁ : ha.rel a₁ a₂ ∨ a₁ = a₂) (h₂ : hb.rel b₁ b₂) :
+  (Prod.lex ha hb).rel (a₁, b₁) (a₂, b₂) := by
+  cases h₁ with
+  | inl h₁ =>
+    apply Prod.Lex.left
+    exact h₁
+  | inr h₁ =>
+    rw [h₁]
+    apply Prod.Lex.right
+    exact h₂
+
+end
+
+section
+
+variable {α β : Type u}
+
+private theorem flush_add_left (a : Nat) {b c : Nat} : b + c + a = b + a + c := by
+  simp only [Nat.add_assoc]
+  rw [Nat.add_comm a c]
+
+theorem mass_lower_bound {x : β} {v : Term α β} (h : Term.Var x ≠ v) (u : Term α β)
+  (θ : Subst α β) : mass u + weight x u * mass (v • θ) ≤ mass (u • (Subst.elementary h * θ)) := by
+  induction u with
+  | Cst c => match θ with
+    | ⟨ θ, _ ⟩ =>
+      suffices p : ∀ n, 0 + 0 * n ≤ 0 from p (mass (map_reduce θ v))
+      intros; simp
+  | Var y => match θ with
+    | ⟨ θ, _ ⟩ =>
+      by_cases p : x = y
+        <;> simp [mass, weight, RSMul.smul, map_reduce, Subst.elementary, HMul.hMul, Mul.mul, comp, p]
+      rw [Nat.one_mul]
+      exact Nat.le.refl
+      simp [Ne.symm p, map_reduce, Nat.zero_le]
+  | Cons l r hl hr =>
+    simp only [mass, weight, subst_cons]
+    simp only [Nat.left_distrib, Nat.right_distrib, ← Nat.add_assoc]
+    simp only [flush_add_left ((weight x r) * mass (v • θ))]
+    simp only [flush_add_left (mass r)]
+    simp only [flush_add_left ((weight x l) * mass (v • θ))]
+    simp only [flush_add_left (mass l)]
+    apply Nat.succ_le_succ
+    rw [Nat.add_assoc]
+    exact Nat.le_of_le_of_le hl hr
+
+theorem weight_nonzero_of_mem_vehicle {x : β} {u : Term α β} (h : x ∈ (𝒱 u : Fintype β)) :
+  weight x u ≠ 0 := by
+  induction u with
+  | Cst _ => exact False.elim <| Fintype.not_mem_empty _ h
+  | Var y =>
+    suffices p : x = y by
+      rw [p]
+      simp [weight]
+    cases h <;> trivial
+  | Cons l r hl hr =>
+    simp only [weight]
+    rw [vehicle_cons, Fintype.mem_union_iff] at h
+    cases h with
+    | inl h => exact Nat.add_ne_zero_of_l_ne_zero <| hl h
+    | inr h => exact Nat.add_ne_zero_of_r_ne_zero <| hr h
+
+end
+
+section
+
+variable {α β : Type u} [Monoid α]
+
+theorem smul_cons_eq {l r : Term α β} {θ : Subst α β} :
+  (Term.Cons l r) • θ = (Term.Cons (l • θ) (r • θ)) :=
+  match θ with
+  | ⟨ θ, hθ ⟩ => rfl
+
+private theorem cons_mgu {l₁ r₁ l₂ r₂ : Term α β} {θ φ : Subst α β}
+  (θ_mgu : is_mgu _ l₁ l₂ θ) (φ_mgu : is_mgu _ (r₁ • θ) (r₂ • θ) φ) :
+  is_mgu _ (Term.Cons l₁ r₁) (Term.Cons l₂ r₂) (θ * φ) := by
+  apply mgu_of_unifies_and_most_general
+  focus
+    simp [smul_cons_eq, ← RAction.smul_mul,
+      unifies_of_mgu θ_mgu, unifies_of_mgu φ_mgu]
+  focus
+    intro
+    simp [smul_cons_eq]
+    intro ⟨ h₁, h₂ ⟩
+    let ⟨ ρ₁, hρ₁ ⟩ := most_general_of_mgu θ_mgu h₁
+    rw [← hρ₁, ← RAction.smul_mul, ← RAction.smul_mul] at h₂
+    let ⟨ ρ₂, hρ₂ ⟩ := most_general_of_mgu φ_mgu h₂
+    exact ⟨ ρ₂, (Monoid.mul_assoc _ _ _ ▸ hρ₂ ▸ hρ₁ ▸ rfl) ⟩
+
+private def rel : WellFoundedRelation (Term α β × Term α β) :=
+  invImage (λ (u, v) => ((𝒱 u ∪ 𝒱 v : Fintype β), (u, v)))
+  <| Prod.lex
+    (Fintype.included_wfRel)
+    (Prod.rprod Term.mass_wfRel Term.mass_wfRel)
+
+abbrev P (x : Option (Subst α β)) (u v : Term α β) := match x with
+  | none => strangers (Subst α β) u v
+  | some θ => is_mgu _ u v θ
+      ∧ (𝒱 θ : Fintype β) ⊆ 𝒱 u ∪ 𝒱 v
+      ∧ vanishing θ
+      ∧ carrier θ ⊆ 𝒱 u ∪ 𝒱 v
+
+private def P_comm (u v : Term α β)
+  : { x // P x u v } → { x // P x v u } := by
+  intro ⟨ x, h ⟩
+  apply Subtype.mk x
+  match x with
+  | none =>
+    simp_all only [strangers_iff_no_unifier]
+    intro θ h'
+    exact h θ h'.symm
+  | some θ =>
+    let ⟨ θ_mgu, θ_vehicle, θ_vanishing, θ_carrier ⟩ := h
+    apply And.intro _ (And.intro _ (And.intro _ _))
+    focus
+      simp only [is_mgu]
+      suffices p : unifiers (Subst α β) v u = unifiers (Subst α β) u v by
+        rw [p]
+        exact θ_mgu
+      funext φ
+      simp [unifiers]
+      apply propext
+      apply Iff.intro
+      intro h; rw [h]
+      intro h; rw [h]
+    focus
+      rw [Fintype.union_comm]
+      exact θ_vehicle
+    focus
+      exact θ_vanishing
+    focus
+      rw [Fintype.union_comm]
+      exact θ_carrier
+
+private theorem decr_left (l₁ r₁ l₂ r₂ : Term α β) :
+  rel.rel (l₁, l₂) (Term.Cons l₁ r₁, Term.Cons l₂ r₂) := by
+  simp [rel, invImage, InvImage]
+  apply lex_of_le_and_lt
+  focus
+    simp [invImage, InvImage, Fintype.included_wfRel]
+    simp only [WellFoundedRelation.rel]
+    simp only [vehicle_cons]
+    suffices h : (𝒱 l₁ ∪ 𝒱 l₂ : Fintype β)
+      ⊆ 𝒱 (Term.Cons l₁ r₁) ∪ 𝒱 (Term.Cons l₂ r₂) by
+      by_cases p : (𝒱 l₁ ∪ 𝒱 l₂ : Fintype β)
+        = 𝒱 (Term.Cons l₁ r₁) ∪ 𝒱 (Term.Cons l₂ r₂)
+      exact Or.inr p
+      exact Or.inl ⟨ h, p ⟩
+    simp only [vehicle_cons]
+    solve_sets
+  focus
+    exact Prod.RProd.intro (mass_decr_l _ _) (mass_decr_l _ _)
+
+private theorem decr_right (l₁ r₁ l₂ r₂ : Term α β) {θ : Subst α β}
+  (θ_vehicle : (𝒱 θ : Fintype β) ⊆ 𝒱 l₁ ∪ 𝒱 l₂)
+  (θ_vanishing : vanishing θ) (θ_carrier : carrier θ ⊆ 𝒱 l₁ ∪ 𝒱 l₂) :
+  rel.rel (r₁ • θ, r₂ • θ) (Term.Cons l₁ r₁, Term.Cons l₂ r₂) := by
+  by_cases h : θ = 1
+  focus
+    rw [h, RAction.smul_one, RAction.smul_one]
+    apply lex_of_le_and_lt
+    focus
+      simp [invImage, InvImage, Fintype.included_wfRel]
+      suffices h : (𝒱 r₁ ∪ 𝒱 r₂ : Fintype β)
+        ⊆ 𝒱 (Term.Cons l₁ r₁) ∪ 𝒱 (Term.Cons l₂ r₂) by
+        by_cases p : (𝒱 r₁ ∪ 𝒱 r₂ : Fintype β)
+          = 𝒱 (Term.Cons l₁ r₁) ∪ 𝒱 (Term.Cons l₂ r₂)
+        exact Or.inr p
+        exact Or.inl ⟨ h, p ⟩
+      simp only [vehicle_cons]
+      solve_sets
+    focus
+      exact Prod.RProd.intro (mass_decr_r _ _) (mass_decr_r _ _)
+  focus
+    apply Prod.Lex.left
+    apply And.intro
+    focus
+      simp only [vehicle_cons]
+      apply Fintype.union_included_iff.2 <| And.intro _ _
+      focus
+        apply Fintype.included_trans (vehicle_on_image Fintype.included_refl r₁)
+        apply Fintype.union_included_iff.2
+          <| And.intro (Fintype.included_trans θ_vehicle _) _
+          <;> solve_sets
+      focus
+        apply Fintype.included_trans (vehicle_on_image Fintype.included_refl r₂)
+        apply Fintype.union_included_iff.2 <| And.intro (Fintype.included_trans θ_vehicle _) _
+          <;> solve_sets
+    focus
+      let ⟨ x, hx ⟩ := (not_one_iff_modifying θ).1 h
+      let not_in_r₁ := vanishing_on_term θ_vanishing hx r₁
+      let not_in_r₂ := vanishing_on_term θ_vanishing hx r₂
+      let not_in_lhs : ¬ x ∈ (𝒱 (r₁ • θ) ∪ 𝒱 (r₂ • θ) : Fintype β) :=
+        λ h => match (Fintype.mem_union_iff _ _ _).1 h with
+          | Or.inl h => not_in_r₁ h
+          | Or.inr h => not_in_r₂ h
+      let in_rhs : x ∈ (𝒱 (Term.Cons l₁ r₁) ∪ 𝒱 (Term.Cons l₂ r₂) : Fintype β) := by
+        simp only [vehicle_cons]
+        have p := carrier_spec.2 hx
+        rw [Fintype.mem_iff_singleton_included]
+        rw [Fintype.mem_iff_singleton_included] at p
+        apply Fintype.included_trans p
+        apply Fintype.included_trans θ_carrier
+        solve_sets
+      exact Fintype.different_if_not_same_element not_in_lhs in_rhs
+
+private theorem prepend_elementary_on_variable_unifier {x : β} {u : Term α β} {θ : Subst α β}
+  (h : Term.Var x ≠ u) (h' : (Term.Var x : Term α β) • θ = u • θ) :
+  θ = (Subst.elementary h) * θ := by
+  apply Subst.ext.2
+  intro y
+  rw [← RAction.smul_mul]
+  by_cases p : y = x
+  focus
+    rw [p, h', Subst.elementary_spec₁]
+  focus
+    rw [Subst.elementary_spec₂]
+    exact p
+
+private def unify_variable_of_not_in_vehicle {x : β} {u : Term α β}
+  (h : ¬ x ∈ (𝒱 u : Fintype β)) : { e : Option (Subst α β) // P e (Term.Var x) u } :=
+  let x_ne_u := (show Term.Var x ≠ u by
+    intro h'
+    rw [← h'] at h
+    apply h
+    apply List.Mem.head);
+  ⟨ some (Subst.elementary x_ne_u), by
+  apply And.intro (mgu_of_unifies_and_most_general _ _)
+    (And.intro _ (And.intro _ _))
+  focus
+    rw [Subst.elementary_spec₁ x_ne_u]
+    rw [elementary_on_not_in_vehicle]
+    exact h
+  focus
+    intro θ hθ
+    apply Exists.intro θ
+    exact Eq.symm <| prepend_elementary_on_variable_unifier x_ne_u hθ
+  focus
+    rw [vehicle_elementary]
+    apply Fintype.included_union_l _ <| Fintype.included_refl
+  focus
+    apply elementary_vanishing
+    exact h
+  focus
+    rw [elementary_carrier]
+    exact Fintype.included_union_r _ <| Fintype.included_refl ⟩
+
+-- Clearly not well written, I sould automate this...
+-- But since I don't do a lot of calculus in the proofs here, I don't feel the need
+-- to spend time writing tactics for numbers.
+private theorem variable_stranger_of_in_vehicle {x : β} {u : Term α β}
+  (h₁ : mass u ≠ 0) (h₂ : x ∈ (𝒱 u : Fintype β)) :
+  strangers (Subst α β) (Term.Var x) u := by
+  have x_ne_u : Term.Var x ≠ u := by
+    intro h
+    apply h₁
+    rw [← h]
+    rfl
+  rw [strangers_iff_no_unifier]
+  intro θ h
+  have p := prepend_elementary_on_variable_unifier x_ne_u h
+  conv at h => rhs; rw [p]
+  have p' := mass_lower_bound x_ne_u u θ
+  conv at p' => rhs; rw [← p]
+  have p'' := Nat.mul_le_mul_right (mass (u • θ))
+    <| Nat.one_le_of_ne_zero
+    <| weight_nonzero_of_mem_vehicle h₂
+  rw [Nat.one_mul] at p''
+  have p₄ := Nat.le_trans p' p''
+  have p₅ : mass u = 0 := by
+    apply byContradiction
+    intro h
+    have p := Nat.lt_of_succ_le <| Nat.one_le_of_ne_zero h
+    have p' := Nat.add_lt_add_right p (weight x u * mass (u • θ))
+    have p''' := Nat.lt_of_lt_of_le p' p₄
+    rw [Nat.zero_add] at p'''
+    exact False.elim <| Nat.not_lt_self _ p'''
+  exact h₁ p₅
+
+theorem strangers_of_left_strangers {l₁ r₁ l₂ r₂ : Term α β} (h : strangers (Subst α β) l₁ l₂) :
+  strangers (Subst α β) (Term.Cons l₁ r₁) (Term.Cons l₂ r₂) := by
+  apply strangers_iff_no_unifier.2
+  intro θ h'
+  apply strangers_iff_no_unifier.1 h θ
+  simp only [subst_cons] at h'
+  apply Term.noConfusion h'
+  exact λ h _ => h
+
+theorem strangers_of_right_strangers {l₁ r₁ l₂ r₂ : Term α β} {θ : Subst α β}
+  (θ_mgu : is_mgu _ l₁ l₂ θ) (h : strangers (Subst α β) (r₁ • θ) (r₂ • θ)) :
+  strangers (Subst α β) (Term.Cons l₁ r₁) (Term.Cons l₂ r₂) := by
+  apply strangers_iff_no_unifier.2
+  intro φ h'
+  suffices h' : l₁ • φ = l₂ • φ ∧ r₁ • φ = r₂ • φ by
+    let ⟨ ρ, hρ ⟩ := most_general_of_mgu θ_mgu h'.1
+    apply strangers_iff_no_unifier.1 h ρ
+    simp only [RAction.smul_mul, hρ]
+    exact h'.2
+  simp only [subst_cons] at h'
+  apply And.intro <;> apply Term.noConfusion h'
+    <;> intros
+          <;> assumption
+
+namespace Robinson
+
+def unify_same {u v : Term α β} (h : u = v) : { e // P e u v } := by
+  apply Subtype.mk (some 1)
+  rw [← h]
+  apply And.intro _ (And.intro _ (And.intro _ _))
+  focus
+    funext θ
+    apply propext
+    suffices p : ∃ ρ, 1 * ρ = θ by
+      simp_all [unifiers, generated_by]
+    apply Exists.intro θ
+    exact Monoid.one_mul _
+  focus
+    rw [vehicle_one]
+    exact Fintype.empty_included _
+  focus
+    exact λ h => False.elim (h rfl)
+  focus
+    rw [is_one_iff_empty_carrier.1 rfl]
+    apply Fintype.empty_included _
+
+def unify_var_cons (x : β) (l r : Term α β) :
+  { e : Option (Subst α β) // P e (Term.Var x) (Term.Cons l r)} :=
+  if p : x ∈ (𝒱 (Term.Cons l r) : Fintype β) then ⟨ none, by
+    apply variable_stranger_of_in_vehicle _ p
+    apply Ne.symm ∘ Nat.ne_of_lt
+      <| Nat.lt_of_lt_of_le (Nat.zero_lt_one) (Nat.le_add_left _ _) ⟩
+  else unify_variable_of_not_in_vehicle p
+
+def unify_var_var (x y : β) :
+  { e : Option (Subst α β) // P e (Term.Var x) (Term.Var y)} :=
+  if p : x = y then unify_same (by rw [p])
+  else by
+    have p' : (Term.Var x : Term α β) ≠ Term.Var y :=
+      λ h => p <| Term.noConfusion h id
+    apply unify_variable_of_not_in_vehicle
+    intro h; apply p; cases h <;> trivial
+
+def unify_var_cst (x : β) (c : α) :
+  { e : Option (Subst α β) // P e (Term.Var x) (Term.Cst c) } := by
+  have p' : (Term.Var x : Term α β) ≠ Term.Cst c := by
+    intro h
+    apply Term.noConfusion h
+  apply unify_variable_of_not_in_vehicle
+  intro h; cases h <;> trivial
+
+def unify_cst_cons (c : α) (l r : Term α β) :
+  { e : Option (Subst α β) // P e (Term.Cst c) (Term.Cons l r) } :=
+  ⟨ none, by
+  apply strangers_iff_no_unifier.2
+  intro ⟨ θ, _ ⟩ h
+  apply Term.noConfusion h ⟩
+
+def unify_cst_cst (a b : α) :
+  { e : Option (Subst α β) // P e (Term.Cst a) (Term.Cst b)} :=
+  if p : a = b then unify_same (by rw [p])
+  else by
+    apply Subtype.mk none
+    apply strangers_iff_no_unifier.2
+    exact λ θ h => p <| match θ with
+    | ⟨ _, _ ⟩ => Term.noConfusion h id
+
+def robinson (u v : Term α β) : { e // P e u v } := match u, v with
+  | Term.Cons l₁ r₁, Term.Cons l₂ r₂ =>
+    match robinson l₁ l₂ with
+    | ⟨ none, h ⟩ => ⟨ none, strangers_of_left_strangers h ⟩
+    | ⟨ some θ, θ_mgu, θ_vehicle, θ_vanishing, θ_carrier ⟩ =>
+      match robinson (r₁ • θ) (r₂ • θ) with
+      | ⟨ none, h ⟩ => ⟨ none, strangers_of_right_strangers θ_mgu h ⟩
+      | ⟨ some φ, φ_mgu, φ_vehicle, φ_vanishing, φ_carrier ⟩ =>
+        ⟨ some (θ * φ),
+          cons_mgu θ_mgu φ_mgu,
+          cons_vehicle_in θ_vehicle φ_vehicle,
+          cons_vanishing θ_vehicle φ_vehicle θ_vanishing φ_vanishing,
+          cons_carrier_in θ_vehicle φ_vehicle θ_vanishing φ_vanishing θ_carrier φ_carrier ⟩
+  | Term.Var x, Term.Cons l r =>
+    unify_var_cons _ _ _
+  | Term.Cons l r, Term.Var x =>
+    P_comm _ _ <| unify_var_cons _ _ _
+  | Term.Var x, Term.Var y =>
+    unify_var_var _ _
+  | Term.Var x, Term.Cst c =>
+    unify_var_cst _ _
+  | Term.Cst c, Term.Var x =>
+    P_comm _ _ <| unify_var_cst _ _
+  | Term.Cst c, Term.Cons l r =>
+    unify_cst_cons _ _ _
+  | Term.Cons l r, Term.Cst c =>
+    P_comm _ _ <| unify_cst_cons _ _ _
+  | Term.Cst a, Term.Cst b =>
+    unify_cst_cst _ _
+termination_by' invImage (λ ⟨ u, v ⟩ => (u, v)) rel
+decreasing_by
+  first
+    | exact decr_left _ _ _ _
+    | apply decr_right <;> assumption
+
+end Robinson
+
+def robinson (u v : Term α β) := (Robinson.robinson u v).1
+
+theorem robinson_eq (u v : Term α β) : robinson u v = match u, v with
+  | Term.Cons l₁ r₁, Term.Cons l₂ r₂ =>
+    match robinson l₁ l₂ with
+    | none => none
+    | some θ => match robinson (r₁ • θ) (r₂ • θ) with
+      | none => none
+      | some φ => some (θ * φ)
+  | Term.Var x, Term.Cons l r =>
+    if p : x ∈ (𝒱 (Term.Cons l r) : Fintype β) then none
+    else subst_simple x (Term.Cons l r)
+  | Term.Cons l r, Term.Var x =>
+    if p : x ∈ (𝒱 (Term.Cons l r) : Fintype β) then none
+    else subst_simple x (Term.Cons l r)
+  | Term.Var x, Term.Var y => some (subst_simple x (Term.Var y))
+  | Term.Var x, Term.Cst c => some (subst_simple x (Term.Cst c))
+  | Term.Cst c, Term.Var x => some (subst_simple x (Term.Cst c))
+  | Term.Cst c, Term.Cons l r => none
+  | Term.Cons l r, Term.Cst c => none
+  | Term.Cst a, Term.Cst b => if a = b then some 1 else none
+  := match u, v with
+  | Term.Cons l₁ r₁, Term.Cons l₂ r₂ => by
+    simp only []
+    conv => lhs; rw [robinson]; unfold Robinson.robinson
+    conv => rhs; rw [robinson]
+    simp only []
+    let o := Robinson.robinson l₁ l₂
+    rw [show Robinson.robinson l₁ l₂ = o from rfl]
+    match o with
+    | Subtype.mk none h => simp only []
+    | ⟨ (some θ), _, _, _, _ ⟩ =>
+      simp only []
+      rw [robinson]
+      let o' := Robinson.robinson (r₁ • θ) (r₂ • θ)
+      rw [show Robinson.robinson (r₁ • θ) (r₂ • θ) = o' from rfl]
+      match o' with
+      | ⟨ none, _ ⟩ => simp
+      | ⟨ some φ, _, _, _, _ ⟩ => simp
+  | Term.Var x, Term.Cons l r => by
+    rw [robinson, Robinson.robinson, Robinson.unify_var_cons]
+    by_cases p : x ∈ (𝒱 (Term.Cons l r) : Fintype β)
+    simp [p]
+    simp [subst_simple, p, unify_variable_of_not_in_vehicle]
+  | Term.Cons l r, Term.Var x => by
+    rw [robinson, Robinson.robinson, Robinson.unify_var_cons]
+    by_cases p : x ∈ (𝒱 (Term.Cons l r) : Fintype β)
+    simp only [p]
+    simp [P_comm]
+    simp only [p]
+    simp [P_comm, subst_simple, unify_variable_of_not_in_vehicle]
+  | Term.Var x, Term.Var y => by
+    rw [robinson, Robinson.robinson, Robinson.unify_var_var]
+    by_cases p : x = y
+    simp [p, subst_simple, Robinson.unify_same]
+    simp [p, subst_simple, unify_variable_of_not_in_vehicle]
+  | Term.Var x, Term.Cst c => by
+    rw [robinson, Robinson.robinson]
+    simp [subst_simple, Robinson.unify_var_cst, unify_variable_of_not_in_vehicle]
+  | Term.Cst c, Term.Var x => by
+    rw [robinson, Robinson.robinson, P_comm]
+    simp [subst_simple, Robinson.unify_var_cst, unify_variable_of_not_in_vehicle]
+  | Term.Cst c, Term.Cons l r => by
+    simp [robinson, Robinson.robinson, Robinson.unify_cst_cons]
+  | Term.Cons l r, Term.Cst c => by
+    simp [robinson, Robinson.robinson, P_comm, Robinson.unify_cst_cons]
+  | Term.Cst a, Term.Cst b => by
+    rw [robinson, Robinson.robinson, Robinson.unify_cst_cst]
+    by_cases p : a = b
+    simp [p]
+    rw [Robinson.unify_same]
+    simp [p]
+
+theorem robinson_spec (u v : Term α β) :
+  match robinson u v with
+  | none => strangers (Subst α β) u v
+  | some θ => is_mgu _ u v θ := by
+  rw [robinson]
+  exact match Robinson.robinson u v with
+  | ⟨ none, h ⟩ => h
+  | ⟨ some _, h, _ ⟩ => h
+
+theorem herbrand (u v : Term α β) :
+  strangers (Subst α β) u v ∨ ∃ θ : Subst α β, is_mgu _ u v θ :=
+  match Robinson.robinson u v with
+  | ⟨ none, p ⟩ => Or.inl p
+  | ⟨ some θ, p, _ ⟩ => Or.inr ⟨ θ, p ⟩
+
+example : robinson (Term.Cons (Term.Var 0) (Term.Var 0) : Term Nat Nat)
+  (Term.Cons (Term.Var 0) (Term.Var 0) : Term Nat Nat) = some 1 := by
+  repeat rw [robinson_eq]; simp
+
+example : robinson (Term.Cons (Term.Var 0) (Term.Var 0) : Term Nat Nat)
+  (Term.Cons (Term.Var 1) (Term.Var 1) : Term Nat Nat) =
+  some (subst_simple 0 (Term.Var 1)) := by
+  repeat rw [robinson_eq]; simp
+
+end
+
